Benchmarks/Liquid-fixpoint/exists_oddity.lean
@@ -3,8 +3,12 @@ import LeanFixpoint
 def existsOddityProp : Prop :=
   ∃ κ0 : Int → Prop,
     (∀ a0 : Int, a0 = 0 → κ0 a0)
-    ∧ (∀ a1 : Int, True → ∀ _x : Int, κ0 a1 → a1 = 0)
-    ∧ (∀ a2 : Int, True → ∀ _x : Int, a2 = 0 → κ0 a2)
+    ∧ (∀ a1 : Int, ∀ _x : Int, κ0 a1 → a1 = 0)
+    ∧ (∀ a2 : Int, ∀ _x : Int, a2 = 0 → κ0 a2)
 
 theorem existsOddityProof : existsOddityProp := by
   solve_fixpoint
+
+theorem test : existsOddityProp := by
+  fusion
+  grind
